Expose the environments in Sem_equiv.

theories/Ext/ExprSem.v
@@ -1,6 +1,8 @@
 Require Import RelationClasses.
 Require Import Morphisms Relations.
+Require Import ExtLib.Data.HList.
 Require Import MirrorCore.SymI.
+Require Import MirrorCore.EnvI.
 Require Import MirrorCore.Ext.Expr.
 
 Set Implicit Arguments.
@@ -11,49 +13,93 @@ Section sem.
   Variable sym : Type.
   Variable RSym_sym : RSym (typD ts) sym.
 
-  Definition Sem_equiv (t : typ) (R : relation (typD ts nil t))
+  Definition Sem_equiv' (t : typ) (R : relation (typD ts nil t)) (tus tvs : tenv typ)
   : relation (expr sym) :=
     fun x y =>
-      forall us tvs,
-        match exprD' us tvs x t , exprD' us tvs y t with
+      forall us : hlist (typD ts nil) tus,
+        match exprD' (join_env us) tvs x t , exprD' (join_env us) tvs y t with
           | None , None => True
           | Some l , Some r => forall vs,
                                  R (l vs) (r vs)
           | _ , _ => False
         end.
 
-  Instance Reflexive_Sem_equiv t Rt (Refl_Rt : Reflexive Rt)
-  : Reflexive (Sem_equiv t Rt).
+  Instance Reflexive_Sem_equiv' t Rt (Refl_Rt : Reflexive Rt) tus tvs
+  : Reflexive (Sem_equiv' t Rt tus tvs).
   Proof.
-    red. red; intros. destruct (exprD' us tvs x t); auto.
+    red. red; intros. destruct (exprD' (join_env us) tvs x t); auto.
   Qed.
 
-  Instance Symmetric_Sem_equiv t Rt (Refl_Rt : Symmetric Rt)
-  : Symmetric (Sem_equiv t Rt).
+  Instance Symmetric_Sem_equiv' t Rt (Refl_Rt : Symmetric Rt) tus tvs
+  : Symmetric (Sem_equiv' t Rt tus tvs).
   Proof.
-    red. unfold Sem_equiv. intros.
-    specialize (H us tvs).
-    destruct (exprD' us tvs x t);
-    destruct (exprD' us tvs y t); intuition.
+    red. unfold Sem_equiv'. intros.
+    specialize (H us).
+    destruct (exprD' (join_env us) tvs x t);
+    destruct (exprD' (join_env us) tvs y t); intuition.
   Qed.
 
-  Instance Transitive_Sem_equiv t Rt (Refl_Rt : Transitive Rt)
-  : Transitive (Sem_equiv t Rt).
+  Instance Transitive_Sem_equiv' t Rt (Refl_Rt : Transitive Rt) tus tvs
+  : Transitive (Sem_equiv' t Rt tus tvs).
   Proof.
-    red. unfold Sem_equiv; red; intros.
-    specialize (H us tvs). specialize (H0 us tvs).
-    destruct (exprD' us tvs x t);
-      destruct (exprD' us tvs y t);
-      destruct (exprD' us tvs z t); auto.
+    red. unfold Sem_equiv'; red; intros.
+    specialize (H us). specialize (H0 us).
+    destruct (exprD' (join_env us) tvs x t);
+      destruct (exprD' (join_env us) tvs y t);
+      destruct (exprD' (join_env us) tvs z t); auto.
     { intros. etransitivity. eapply H. eauto. }
     { intuition. }
   Qed.
 
-  Definition Sem_ext (t : typ) (P : typD ts nil t -> Prop) (Q : Prop)
+  Definition Sem_equiv (t : typ) (R : relation (typD ts nil t)) (us vs : env (typD ts))
+  : relation (expr sym) :=
+    fun x y =>
+      match exprD us vs x t , exprD us vs y t with
+        | None , None => True
+        | Some l , Some r => R l r
+        | _ , _ => False
+      end.
+
+  Instance Reflexive_Sem_equiv t Rt (Refl_Rt : Reflexive Rt) us vs
+  : Reflexive (Sem_equiv t Rt us vs).
+  Proof.
+    red. red; intros.
+    destruct (exprD us vs x t); auto.
+  Qed.
+
+  Instance Symmetric_Sem_equiv t Rt (Refl_Rt : Symmetric Rt) us vs
+  : Symmetric (Sem_equiv t Rt us vs).
+  Proof.
+    red. unfold Sem_equiv. intros.
+    destruct (exprD us vs x t);
+    destruct (exprD us vs y t); intuition.
+  Qed.
+
+  Instance Transitive_Sem_equiv t Rt (Refl_Rt : Transitive Rt) us vs
+  : Transitive (Sem_equiv t Rt us vs).
+  Proof.
+    red. unfold Sem_equiv.
+    intros.
+    destruct (exprD us vs x t);
+      destruct (exprD us vs y t);
+      destruct (exprD us vs z t); auto.
+    { intros. etransitivity. eapply H. eauto. }
+    { intuition. }
+  Qed.
+
+  Definition Sem_ext (t : typ) (P : typD ts nil t -> Prop) (Q : Prop) us vs
   : expr sym -> Prop :=
     fun e =>
-      forall us tvs,
-        match exprD' us tvs e t with
+      match exprD us vs e t with
+        | Some val => P val
+        | None => Q
+      end.
+
+  Definition Sem_ext' (t : typ) (P : typD ts nil t -> Prop) (Q : Prop) tus tvs
+  : expr sym -> Prop :=
+    fun e =>
+      forall us : hlist (typD ts nil) tus,
+        match exprD' (join_env us) tvs e t with
           | Some val =>
             forall vs, P (val vs)
           | None => Q
